src/program_proof/simplefs/bitmap_proof.v
@@ -1,0 +1,392 @@
+From Perennial.program_proof Require Import proof_prelude.
+From Perennial.program_proof Require Import disk_prelude.
+From Perennial.goose_lang.lib Require Import typed_slice.
+From Perennial.program_proof Require Import disk_lib.
+From Perennial.Helpers Require Import bytes.
+
+From Goose.github_com Require Import tchajed.simplefs.
+
+#[local] Unset Printing Projections.
+
+Definition BlkBits: Z := (4096*8).
+
+Section proof.
+Context `{!heapGS Σ}.
+
+Definition is_block_typed (s: Slice.t) (dq: dfrac) (block: Block) :=
+  own_slice_small s byteT dq (vec_to_list block).
+
+Lemma is_block_to_typed s dq block :
+  is_block s dq block = is_block_typed s dq block.
+Proof. reflexivity. Qed.
+
+Definition block_has_bits (block: Block) (bits: list bool) :=
+  Z.of_nat (length bits) = BlkBits ∧
+  ∀ (i: nat) (bit: bool),
+  bits !! i = Some bit →
+  ∃ (b: u8), vec_to_list block !! (i `div` 8)%nat = Some b ∧
+             Z.testbit (uint.Z b) (i `mod` 8)%nat = bit.
+
+Definition block_to_bits (block: Block): list bool :=
+  concat (byte_to_bits <$> vec_to_list block).
+
+Definition length_uniform {A: Type} (l: list (list A)) (n: nat) :=
+  ∀ i x, l !! i = Some x → length x = n.
+
+Lemma length_uniform_app_inv {A} (a: list A) (l: list (list A)) n :
+  length_uniform (a :: l) n →
+  length a = n ∧ length_uniform l n.
+Proof.
+  rewrite /length_uniform.
+  intros Hlen.
+  pose proof (Hlen 0%nat a) as H; simpl in H.
+  split; auto.
+  intros.
+  pose proof (Hlen (S i)). auto.
+Qed.
+
+Lemma length_concat_uniform {A: Type} (l: list (list A)) (n: nat) :
+  length_uniform l n →
+  length (concat l) = (length l * n)%nat.
+Proof.
+  intros Hlen.
+  induction l; simpl; auto.
+  apply length_uniform_app_inv in Hlen as [Ha Hlen].
+  intuition.
+  autorewrite with len.
+  rewrite H //.
+  lia.
+Qed.
+
+Lemma lookup_concat_uniform {A: Type} (l: list (list A)) (n: nat) :
+  length_uniform l n →
+  n ≠ 0%nat →
+  ∀ i, concat l !! i =
+         (l !! (i `div` n)%nat) ≫= λ (ll: list A), ll !! (i `mod` n)%nat.
+Proof.
+  intros Hlen Hn.
+  induction l.
+  - simpl. intros. rewrite lookup_nil //.
+  - apply length_uniform_app_inv in Hlen as [Ha Hlen].
+    simpl. intros i.
+    destruct (decide (i < n)%nat).
+    + rewrite lookup_app_l; [ | lia ].
+      rewrite Nat.div_small // /=.
+      rewrite Nat.mod_small //.
+    + rewrite lookup_app_r; [ | lia ].
+      rewrite IHl //.
+      rewrite Ha.
+      replace i with (1*n + (i-n))%nat at 2 by lia.
+      rewrite Nat.div_add_l; [ | lia ].
+      simpl.
+      f_equal.
+      f_equal.
+      admit. (* nonlinear arith goal (mod and minus) *)
+Admitted.
+
+Hint Unfold BlkBits : word.
+Hint Unfold block_bytes : word.
+
+Lemma byte_to_bits_uniform block :
+  length_uniform (byte_to_bits <$> block) 8%nat.
+Proof.
+  intros i x H.
+  fmap_Some in H as b.
+  len.
+Qed.
+
+Hint Resolve byte_to_bits_uniform : core.
+
+Lemma block_to_bits_length block :
+  length (block_to_bits block) = Z.to_nat BlkBits.
+Proof.
+  rewrite /block_to_bits.
+  rewrite (length_concat_uniform _ 8%nat).
+  { len. }
+  apply byte_to_bits_uniform.
+Qed.
+
+Hint Rewrite block_to_bits_length : len.
+
+Lemma byte_to_bits_lookup_Some (bytes: list u8) (i: nat) (bit: bool) :
+  concat (byte_to_bits <$> bytes) !! i = Some bit →
+  ∃ (b: u8), bytes !! (i `div` 8)%nat = Some b ∧
+             byte_to_bits b !! (i `mod` 8)%nat = Some bit.
+Proof.
+  intros Hlookup.
+  erewrite lookup_concat_uniform in Hlookup; eauto.
+  apply bind_Some in Hlookup as [bits [Hlookup' Hlookup_bit]].
+  fmap_Some in Hlookup' as b. exists b.
+  eauto.
+Qed.
+
+Lemma block_has_to_bits block:
+  block_has_bits block (block_to_bits block).
+Proof.
+  split.
+  + len.
+  + intros ?? Hlookup.
+    destruct (list_lookup_lt _ block (i `div` 8)) as [b Hlookup2].
+    { apply lookup_lt_Some in Hlookup.
+      autorewrite with len in Hlookup.
+      apply Nat.Div0.div_lt_upper_bound.
+      move: Hlookup; len. }
+    exists b; split; [ by auto | ].
+    apply byte_to_bits_lookup_Some in Hlookup as [b' [Hlookup' Hlookup_bit]].
+    assert (b = b') by congruence; subst.
+    rewrite /byte_to_bits in Hlookup_bit.
+    fmap_Some in Hlookup_bit.
+    apply lookup_seqZ in Hlookup_bit; intuition subst.
+    f_equal; lia.
+Qed.
+
+Lemma block_to_bits_ok block :
+  ∀ bits, block_has_bits block bits ↔ bits = block_to_bits block.
+Proof.
+  intros. split.
+  - intros H.
+    destruct H as [Hlen Hbits].
+    eapply list_eq_same_length; auto.
+    { len. }
+    len. intros ??? Hi Hlookup1 Hlookup2.
+    apply Hbits in Hlookup1 as [b [Hlookup1 Htestbit]].
+    rewrite /block_to_bits in Hlookup2.
+    (* this proof is harder than it's worth *)
+    admit.
+  - intros ->.
+    apply block_has_to_bits.
+Abort.
+
+Definition own_blockBitmap (bb: val) (block: Block) (bits: list bool): iProp Σ :=
+  ∃ (s: Slice.t), ⌜bb = (slice_val s, #())%V⌝ ∗
+                   ⌜Z.of_nat (length bits) = BlkBits⌝ ∗
+                   is_block s (DfracOwn 1) block ∗
+                   ⌜bits = block_to_bits block⌝.
+
+Lemma wp_newBlockBitmap s block :
+  {{{ is_block s (DfracOwn 1) block }}}
+    newBlockBitmap (slice_val s)
+  {{{ v bits, RET v; own_blockBitmap v block bits }}}.
+Proof.
+  (*@ func newBlockBitmap(block disk.Block) blockBitmap {                     @*)
+  (*@     return blockBitmap{block: block}                                    @*)
+  (*@ }                                                                       @*)
+  iIntros (Φ) "Hpre HΦ".
+  wp_rec.
+  wp_pures.
+  iApply ("HΦ" $! _ (block_to_bits block)).
+  iModIntro.
+  iFrame.
+  iPureIntro.
+  split; [ by eauto | ].
+  split.
+  - len.
+  - (* apply block_has_to_bits. *) auto.
+Qed.
+
+Lemma symex_wp_blockBitmap__Set s (bytes: list u8) (i : u64) :
+  {{{ own_slice_small s byteT (DfracOwn 1) bytes ∗ ⌜length bytes = 4096%nat⌝ ∗ ⌜uint.Z i < BlkBits⌝ }}}
+    blockBitmap__Set (s, #())%V #i
+  {{{ (b: w8), RET #();
+      ⌜bytes !! (uint.nat i `div` 8)%nat = Some b⌝ ∗
+      own_slice_small s byteT (DfracOwn 1)
+                 (<[(uint.nat i `div` 8)%nat:=word.or b
+                                                    (word.slu
+                                                       (W8 1)
+                                                       (W8 (uint.Z i `mod` 8)))]>
+               bytes) }}}.
+Proof.
+  iIntros (Φ) "Hpre HΦ". iDestruct "Hpre" as "(Hbb & %Hbytelen & %Hbound)".
+  wp_rec. wp_pures.
+  rewrite bool_decide_eq_false_2.
+  2: {
+    change (word.mul (W64 4096) (W64 8)) with (W64 32768).
+    word.
+  }
+  wp_pures.
+  assert (exists b:u8, bytes !! (uint.nat i / 8)%nat = Some b) as [b Hlookup].
+  { apply list_lookup_lt. apply Nat.Div0.div_lt_upper_bound. len. }
+  word_cleanup.
+  wp_apply (wp_SliceGet with "[$Hbb]").
+  { word_cleanup.
+    rewrite Z2Nat.inj_div //. word. }
+  iIntros "Hbb".
+  wp_pures.
+  wp_apply (wp_SliceSet with "[$Hbb]").
+  { iPureIntro. apply lookup_lt_is_Some.
+    word_cleanup. rewrite -> Z2Nat.inj_div by word.
+    apply Nat.Div0.div_lt_upper_bound. len. }
+  iIntros "Hbb".
+  word_cleanup.
+  rewrite -> Z2Nat.inj_div by word. change (Z.to_nat 8) with 8%nat.
+  wp_pures.
+  iModIntro.
+  iApply "HΦ".
+  iSplit.
+  { iPureIntro. eauto. }
+  iFrame.
+Qed.
+
+Local Ltac Zify.zify_post_hook ::= Z.div_mod_to_equations.
+
+Lemma own_slice_small_to_block s dq (l: list u8) :
+  length l = Z.to_nat 4096 →
+  own_slice_small s byteT dq l = is_block s dq (list_to_block l).
+Proof.
+  intros Hlen.
+  rewrite is_block_to_typed /is_block_typed.
+  rewrite list_to_block_to_list //.
+Qed.
+
+Lemma Some_inv {A} (a b: A) : Some a = Some b → a = b.
+Proof. inversion 1; auto. Qed.
+
+Lemma Some_eq_iff {A} (a b: A) : Some a = Some b ↔ a = b.
+Proof. split; [ apply Some_inv | congruence ]. Qed.
+
+Transparent w8_instance.w8.
+Lemma set_bit_get (b: w8) (i: u64) bit :
+  byte_to_bits (word.or b (word.slu (W8 1) (W8 (uint.Z i `mod` 8))))
+  !! Z.to_nat (uint.Z i `mod` 8) = Some bit → true = bit.
+Proof.
+    byte_cases b; bit_off_cases (uint.Z i `mod` 8); compute;
+      intros H%Some_inv; exact H.
+Qed.
+
+Lemma byte_to_bits_lookup (b: u8) (i: nat) :
+  byte_to_bits b !! (i `mod` 8)%nat =
+    Some (Z.testbit (uint.Z b) (i `mod` 8)%nat ).
+Proof.
+  rewrite /byte_to_bits.
+  rewrite list_lookup_fmap.
+  assert (seqZ 0 8 !! (i `mod` 8)%nat = Some (i `mod` 8)).
+  { apply lookup_seqZ.
+    rewrite Nat2Z.inj_mod.
+    split; lia. }
+  rewrite !Nat2Z.inj_mod.
+  rewrite H.
+  reflexivity.
+Qed.
+
+Lemma set_get_bit_ne (i : w64) (b : w8) (i' : nat) (bit1 bit2 : bool) :
+  (Z.to_nat (uint.Z i `mod` 8) ≠ i' `mod` 8)%nat →
+  byte_to_bits (word.or b (word.slu (W8 1) (W8 (uint.Z i `mod` 8))))
+    !! (i' `mod` 8)%nat = Some bit2
+  → byte_to_bits b !! (i' `mod` 8)%nat = Some bit1 → bit1 = bit2.
+Proof.
+  clear Σ heapGS0.
+  intros Hmodneq.
+  rewrite byte_to_bits_lookup.
+  rewrite byte_to_bits_lookup.
+  rewrite !Some_eq_iff. intros <- <-.
+  move: Hmodneq.
+  assert (i' `mod` 8 < 8)%nat as Hbound.
+  { pose proof (Nat.mod_bound_pos i' 8%nat). lia.
+  }
+  bit_off_cases (i' `mod` 8)%nat;
+    bit_off_cases (uint.Z i `mod` 8);
+    try (intros H; compute in H; exfalso; congruence);
+    byte_cases b;
+    compute;
+    auto.
+Qed.
+
+Opaque w8_instance.w8.
+
+Lemma byte_bit_update (data : list u8) (i : w64) (b : w8) :
+  data !! (uint.nat i `div` 8)%nat = Some b
+  → <[uint.nat i:=true]> (concat (byte_to_bits <$> data)) =
+      concat
+        (byte_to_bits <$>
+          <[(uint.nat i `div` 8)%nat
+            :=word.or b
+                (word.slu (W8 1) (W8 (uint.Z i `mod` 8)))]>
+            data).
+Proof.
+  intros Hbyte_lookup.
+  eapply (list_eq_same_length _ _ (length data * 8)%nat); [ | | ].
+  { erewrite -> !length_concat_uniform by eauto.
+    len. }
+  { autorewrite with len.
+    erewrite -> !length_concat_uniform by eauto.
+    len. }
+  intros i' bit1 bit2 Hbound Hlookup1 Hlookup2.
+  apply byte_to_bits_lookup_Some in Hlookup2 as [b' [Hlookupb' Hb']].
+
+  destruct (decide (uint.nat i `div` 8 = i' `div` 8)%nat).
+  - (* same byte *)
+    rewrite -e in Hlookupb'.
+    rewrite list_lookup_insert in Hlookupb'.
+    2: {
+      apply lookup_lt_Some in Hbyte_lookup.
+      word.
+    }
+
+    destruct (decide (uint.nat i = i')); subst.
+    + (* same bit *)
+      rewrite list_lookup_insert in Hlookup1.
+      2: {
+        erewrite length_concat_uniform; [ | eauto ]. len.
+      }
+      inversion Hlookup1; subst.
+      inversion Hlookupb'; subst; clear Hlookupb'.
+      move: Hb'.
+      replace (uint.nat i `mod` 8)%nat with (Z.to_nat (uint.Z i `mod` 8)).
+      2: {
+        rewrite Z2Nat.inj_mod //; word.
+      }
+      apply set_bit_get.
+    + (* same byte but different bit *)
+      rewrite list_lookup_insert_ne // in Hlookup1.
+      apply byte_to_bits_lookup_Some in Hlookup1 as [b'' [Hlookupb'' Hb'']].
+      assert (b = b'') by congruence; subst.
+      inversion Hlookupb'; subst; clear Hlookupb'.
+
+      eapply set_get_bit_ne; eauto.
+      rewrite Z2Nat.inj_mod //; try word.
+      change (Z.to_nat 8) with 8%nat.
+      intros Heq.
+      contradiction n.
+      admit.
+
+  - assert (uint.nat i ≠ i') by congruence.
+    rewrite list_lookup_insert_ne // in Hlookup1.
+    rewrite list_lookup_insert_ne // in Hlookupb'.
+    apply byte_to_bits_lookup_Some in Hlookup1 as [b'' [Hlookupb'' Hb'']].
+    congruence.
+
+Admitted.
+
+Lemma wp_blockBitmap__Set v block bits (i : u64) :
+  {{{ own_blockBitmap v block bits ∗ ⌜uint.Z i < BlkBits⌝ }}}
+    blockBitmap__Set v #i
+  {{{ block', RET #(); own_blockBitmap v block' (<[uint.nat i := true]> bits) }}}.
+Proof.
+  (*@ func (b blockBitmap) Set(i uint64) {                                    @*)
+  (*@     if i >= BLK_BITS {                                                  @*)
+  (*@         panic("out of bounds")                                          @*)
+  (*@     }                                                                   @*)
+  (*@     byteIndex := i / 8                                                  @*)
+  (*@     bitIndex := i % 8                                                   @*)
+  (*@     b.block[byteIndex] |= 1 << bitIndex                                 @*)
+  (*@ }                                                                       @*)
+  iIntros (Φ) "Hpre HΦ". iDestruct "Hpre" as "[Hbb %Hbound]".
+  iDestruct "Hbb" as (s) "(-> & %Hlen & Hblock & %Hbits)".
+  wp_apply (symex_wp_blockBitmap__Set with "[$Hblock]").
+  { iPureIntro. len. }
+  iIntros (b) "[%Hbyte_lookup Hbb]".
+  rewrite own_slice_small_to_block; [ | len ].
+  iApply "HΦ".
+  iFrame "Hbb".
+
+  iPureIntro.
+  split; [ done | ].
+  split; [ by len | ].
+
+  rewrite /block_to_bits.
+  rewrite list_to_block_to_list; [ | len ].
+  rewrite -byte_bit_update //.
+  subst. auto.
+Qed.
+
+End proof.
